some more support for arrays and a new q	uicksort example using arrays

examples/separationLogic/src/holfoot/AssembleHolfootParser.sig
@@ -1,6 +1,6 @@
 signature AssembleHolfootParser =
 sig
-  val raw_read_stream : TextIO.instream -> Parsetree.p_program
-  val raw_read_file : string -> Parsetree.p_program
+  val raw_read_stream : TextIO.instream -> Parsetree.p_top
+  val raw_read_file : string -> Parsetree.p_top
   val print_parse_error : string -> unit;
 end
