examples/separationLogic/src/holfoot/holfootLib.sml
@@ -1,6 +1,7 @@
 structure holfootLib :> holfootLib =
 struct
 
+
 (*
 quietdec := true;
 use (Globals.HOLDIR ^ "/examples/separationLogic/src/holfoot/header.sml");
@@ -93,6 +94,16 @@ fun holfoot_term_to_string t =
        stringLib.fromHOLstring (dest_holfoot_var t)
    else term_to_string t
 
+
+fun is_no_proper_diseq thm = 
+   let
+      val (t1, t2) = dest_eq (dest_neg (concl thm));
+   in
+      (same_const t1 numSyntax.zero_tm) orelse
+      (same_const t2 numSyntax.zero_tm)
+   end handle HOL_ERR _ => true;
+
+
 structure holfoot_base_param = 
 struct
    val exp_to_string = holfoot_term_to_string;
@@ -104,15 +115,6 @@ struct
         REWRITE_RULE [holfoot_separation_combinator_def] GET_VAR_RES_COMBINATOR___holfoot_separation_combinator,
         IS_SEPARATION_COMBINATOR___FINITE_MAP, IS_SEPARATION_COMBINATOR___holfoot_separation_combinator,
         REWRITE_RULE [holfoot_separation_combinator_def] IS_SEPARATION_COMBINATOR___holfoot_separation_combinator];
-   val LENGTH_NIL_GSYM = CONV_RULE ((QUANT_CONV o LHS_CONV) SYM_CONV) LENGTH_NIL
-
-   fun is_no_proper_diseq thm = 
-   let
-      val (t1, t2) = dest_eq (dest_neg (concl thm));
-   in
-      (same_const t1 numSyntax.zero_tm) orelse
-      (same_const t2 numSyntax.zero_tm)
-   end handle HOL_ERR _ => true;
 
    fun LENGTH_EQ_conv tt =
    let
@@ -168,7 +170,15 @@ struct
         BUTLAST, LAST, NOT_NULL_SNOC,
         FIRSTN_LENGTH_ID_EVAL, BUTFIRSTN_LENGTH_NIL_EVAL,
         holfoot_var_res_map_REWRITES,
-        holfoot_separation_combinator_def
+        holfoot_separation_combinator_def,
+        REPLACE_ELEMENT_compute,
+        REPLACE_ELEMENT_SEM, REPLACE_ELEMENT_DEF,
+        EL_REPLACE_ELEMENT,
+
+        SUB1, arithmeticTheory.ADD1, arithmeticTheory.NOT_LESS,
+        arithmeticTheory.NOT_LESS_EQUAL,
+        arithmeticTheory.GREATER_DEF,
+        arithmeticTheory.GREATER_EQ
      ]])
 
    val varlist_rwts = [holfoot___varlist_update_NO_VAR_THM];
@@ -203,8 +213,43 @@ fun array_bound_DECIDE context t =
    end
 *)
 
+val sub_add_simp = prove (``(((x:num) + (c1:num)) - (x + c2)) = (c1 - c2)``, DECIDE_TAC)
+
+val arith_simp_ss = 
+   std_ss ++ simpLib.merge_ss [
+     (numSimps.ARITH_DP_FILTER_ss is_no_proper_diseq),
+     simpLib.rewrites [arithmeticTheory.ADD1, SUB1,
+      sub_add_simp]]
+
+fun holfoot_arith_simp_CONV context t = 
+   SIMP_CONV arith_simp_ss context t
+  handle UNCHANGED => REFL t
+
+
 fun array_bound_DECIDE context t = 
-   EQT_ELIM (SIMP_CONV arith_ss context t);
+   (EQT_ELIM (holfoot_arith_simp_CONV context t));
+
+fun prove_in_array_bound context ec (ec', nc') =
+   let
+      val thm_t = mk_conj (
+                      numSyntax.mk_leq (ec', ec),
+                      numSyntax.mk_less (ec, numSyntax.mk_plus (ec', nc')))
+   in 
+      array_bound_DECIDE context thm_t
+   end;
+
+
+fun prove_in_interval_bound context ec (ec2, ec3) =
+   let
+      val thm_t = mk_conj (
+                      numSyntax.mk_leq (ec2, ec),
+                      numSyntax.mk_leq (ec, ec3))
+   in 
+      array_bound_DECIDE context thm_t
+   end;
+
+fun prove_in_array_interval_bound true = prove_in_interval_bound
+  | prove_in_array_interval_bound false = prove_in_array_bound
 
 
 (******************************************************************************)
@@ -292,7 +337,7 @@ let
    
    val found_opt = first_opt (unequal_opt_pred c1 c2) context
    val found_opt = if isSome (found_opt) then found_opt else 
-          SOME (EQT_ELIM (numLib.ARITH_CONV (mk_neg (mk_eq (c1, c2)))))
+          SOME (EQT_ELIM (holfoot_arith_simp_CONV context (mk_neg (mk_eq (c1, c2)))))
    val _ = if no_thm then raise var_res_implies_unequal_found_expn else ();
    val thm_context = valOf found_opt;
 
@@ -399,18 +444,20 @@ end handle HOL_ERR _ => []
          | UNCHANGED => []
 
 
-fun holfoot_implies_in_heap_GENERATE___data_array tL context sfb tt =
+fun holfoot_implies_in_heap_GENERATE___data_array_interval tL context sfb tt =
 let
-   val (e,n,data) = dest_holfoot_ap_data_array tt;
-   val ec = dest_var_res_exp_const e
-   val nc = dest_var_res_exp_const n
-   val base_thm = ISPECL [ec, nc, data, sfb]
-           holfoot_ap_data_array___implies_in_heap___COMPUTE
+   val (is_interval, (e1,e2,data)) = dest_holfoot_ap_data_array_interval tt;
+   val c1 = dest_var_res_exp_const e1
+   val c2 = dest_var_res_exp_const e2
+   val base_thm = ISPECL [c1, c2, data, sfb]
+          (if (is_interval) then
+              holfoot_ap_data_interval___implies_in_heap___COMPUTE
+           else
+              holfoot_ap_data_array___implies_in_heap___COMPUTE);
 
-   val ec_vars = FVL [ec] empty_tmset;
-
+   val ec_vars = FVL [c1,c2] empty_tmset;
    fun term_filter t = (type_of t = numSyntax.num) andalso
-       not (HOLset.isEmpty (HOLset.intersection (FVL [t] empty_tmset, ec_vars)))
+       ((is_var t) orelse (not (HOLset.isEmpty (HOLset.intersection (FVL [t] empty_tmset, ec_vars)))))
    val constL = 
        HOLset.listItems (
          foldl (fn (l,s) => HOLset.addList (s,l)) empty_tmset
@@ -438,7 +485,7 @@ fun holfoot_implies_in_heap_GENERATE tL context sfb tt =
        holfoot_implies_in_heap_GENERATE___data_list_seg,
        holfoot_implies_in_heap_GENERATE___tree,
        holfoot_implies_in_heap_GENERATE___data_tree,
-       holfoot_implies_in_heap_GENERATE___data_array])
+       holfoot_implies_in_heap_GENERATE___data_array_interval])
 
 
 fun holfoot_implies_in_heap___or_null___EXTEND_BAG sfb2 thm =
@@ -503,40 +550,75 @@ in
  thm3
 end;
 
-fun holfoot_implies_GENERATE___data_array ss context (wpb, rpb) sfb =
+fun holfoot_implies_GENERATE___data_array_interval ss context (wpb, rpb) sfb =
 let
    val sfs = fst (dest_bag sfb);
    fun indexes n p [] = []
      | indexes n p (e::es) =
-         if (p e) then n::(indexes (n + 1) p es) else
-                          (indexes (n + 1) p es);
+         let
+            val r_opt = p (e);
+            val l = indexes (n + 1) p es;
+         in
+            if (isSome  r_opt) then ((n, (valOf r_opt))::l) else l
+         end;
 
    fun my_holfoot_ap_data_array___pred tt =
    let
-      val (_, n, dataL) = dest_holfoot_ap_data_array tt;
+      val (is_interval, (e1, e2, dataL)) = dest_holfoot_ap_data_array_interval tt;
       val (td, _) = listSyntax.dest_cons dataL;
       val (_, d) = pairSyntax.dest_pair td;      
-      val length_const0 = mk_comb (holfoot_exp_const_term,
-              (listSyntax.mk_length d))
-      val length_const = rhs (concl (VAR_RES_PROP_REWRITE_CONV ss context length_const0)) handle UNCHANGED => length_const0
+      val length_d = listSyntax.mk_length d;
+      val length_const = mk_comb (holfoot_exp_const_term, length_d);
+
+      (*check, whether this lenght should be introduced*)
+      val _ = if is_interval then
+                 let
+                    val c1 = dest_var_res_exp_const e1;
+                    val c2 = dest_var_res_exp_const e2;
+                    val b_t = mk_eq (length_d, 
+                        numSyntax.mk_minus (numSyntax.mk_suc c2, c1))
+                    val is_new = ((array_bound_DECIDE context b_t);false)
+                        handle HOL_ERR _ => true;
+                 in
+                    if (is_new) then () else Feedback.fail()
+                 end
+              else (
+                 (* its an array*)
+                 if (exists (is_var_res_prop_equal_sym e2 length_const) sfs) then
+                    (Feedback.fail ())
+                 else if not (is_var_res_exp_const e2) then () else
+                 let                  
+                    val c2 = dest_var_res_exp_const e2;
+                    val b_t = mk_eq (length_d, c2)
+                    val is_new = ((array_bound_DECIDE context b_t);false)
+                        handle HOL_ERR _ => true;
+                 in
+                    if (is_new) then () else Feedback.fail()
+                 end)
    in
-      (not (is_var_res_exp_const n) orelse
-       not (aconv length_const n)) andalso
-      (not (exists (is_var_res_prop_equal_sym n length_const) sfs))
-   end handle HOL_ERR _ => false;
+      SOME (is_interval)
+   end handle HOL_ERR _ => NONE;
 
    val iL = indexes 0 my_holfoot_ap_data_array___pred sfs;
-   val inf_thm = ISPECL [wpb, rpb] holfoot_ap_data_array___var_res_prop_implies___length_eq
 
-   fun process_index i = 
+   fun process_index (i, is_interval) = 
    let
        val sfb_thm = BAG_RESORT_CONV [i] sfb;
-       val xthm0 = PART_MATCH (rand o rator o snd o dest_imp)
-            inf_thm (rhs (concl sfb_thm));
-       val xthm1 = var_res_precondition_prove xthm0;
-       val xthm2 = CONV_RULE (RATOR_CONV (RAND_CONV (K (GSYM sfb_thm)))) xthm1
+       val xthm0 = if (is_interval) then
+            (PART_MATCH (rand o rator) 
+                (ISPECL [wpb, rpb] holfoot_ap_data_interval___var_res_prop_implies___length_eq)
+                (rhs (concl sfb_thm))) else 
+            let
+               val ythm0 = PART_MATCH (rand o rator o snd o dest_imp) 
+                   (ISPECL [wpb, rpb] holfoot_ap_data_array___var_res_prop_implies___length_eq)
+                    (rhs (concl sfb_thm));
+               val ythm1 = var_res_precondition_prove ythm0;
+            in
+               ythm1
+            end;
+       val xthm1 = CONV_RULE (RATOR_CONV (RAND_CONV (K (GSYM sfb_thm)))) xthm0
    in
-      [xthm2]
+      [xthm1]
    end handle HOL_ERR _ => [];
 in
    flatten (map process_index iL)
@@ -646,6 +728,14 @@ local
 
 in
 
+(*
+   val context = map ASSUME (fst (top_goal()))
+   val tt = find_term is_VAR_RES_FRAME_SPLIT (snd (top_goal ()))
+
+   val (f, _, wpbrpb, _, sfb_context, sfb_split, sfb_imp, _) = dest_VAR_RES_FRAME_SPLIT tt
+   val (wpb,rpb) = pairSyntax.dest_pair wpbrpb
+   val sfb = sfb_context
+*)
 
 fun holfoot___var_res_prop_implies___GENERATE tL ss context 
     (f, wpb, rpb, sfb) =
@@ -669,7 +759,7 @@ let
    val res2L = mapfilter (mk_equal___in_heap_or_null___in_heap_or_null wpb rpb) implies_in_heap_pairL
 
 
-   val res3L = holfoot_implies_GENERATE___data_array ss context (wpb,rpb) sfb'
+   val res3L = holfoot_implies_GENERATE___data_array_interval ss context (wpb,rpb) sfb'
 
    val res = flatten [res1L, res2L, res3L]
    val res2 = map (CONV_RULE (RATOR_CONV (RAND_CONV (K (GSYM sfb_thm))))) res
@@ -1015,19 +1105,14 @@ local
    val _ = computeLib.add_thms char_eq_thms apply_compset
    val _ = computeLib.add_thms [FAPPLY_FUPDATE_THM, holfoot_tag_11] apply_compset
 
-
-   fun search_fun_array context ec n ttt =
+   fun search_fun_array_interval context ec n ttt =
        let
-          val (e',n',_) = dest_holfoot_ap_data_array ttt
+          val (is_interval, (e',n',_)) = dest_holfoot_ap_data_array_interval ttt
           val nc' = dest_var_res_exp_const n';
           val ec' = dest_var_res_exp_const e';
-
-          val thm_t = mk_conj (
-                         numSyntax.mk_leq (ec', ec),
-                         numSyntax.mk_less (ec, numSyntax.mk_plus (ec', nc')))
-          val thm = array_bound_DECIDE context thm_t
+          val thm = prove_in_array_interval_bound is_interval context ec (ec',nc')
        in          
-          SOME (n, thm, ttt)
+          SOME (n, thm, ttt, is_interval)
        end handle HOL_ERR _ => NONE;
 
 in
@@ -1078,23 +1163,24 @@ in
 end;
 
 (*
+   val context = map ASSUME (fst (top_goal ()))
    val tt = find_term is_VAR_RES_COND_HOARE_TRIPLE (snd (top_goal ()))
 *)
 fun HOLFOOT_INFERENCE___field_lookup___main_array___CONSEQ_CONV context tt =
 let
-   (*destruct and search for points to*)
+   (*destruct and search for array / interval*)
    val (p1,_,_,pre,_) = dest_VAR_RES_COND_HOARE_TRIPLE___FIRST_COMMAND tt;
    val (v, e, tag_t) = dest_holfoot_prog_field_lookup p1
    val ec = dest_var_res_exp_const e;
 
    val (_, _, _, _, sfs) = dest_var_res_prop___propL pre;
-   val found_opt = first_opt (search_fun_array context ec) sfs;
+   val found_opt = first_opt (search_fun_array_interval context ec) sfs;
    val _ = if isSome found_opt then () else raise UNCHANGED;
-   val (n, index_thm, sf) = valOf found_opt;
+   val (n, index_thm, sf, is_interval) = valOf found_opt;
 
 
    (*find the apropriate instantiations*)
-   val (_,_,data) = dest_holfoot_ap_data_array sf;
+   val (_, (_,_,data)) = dest_holfoot_ap_data_array_interval sf;
    val (dataL, _) = listSyntax.dest_list data 
    val t_data = tryfind (fn dt => let val (tag, dl) = pairSyntax.dest_pair dt in
                    if (aconv tag tag_t) then dl else Feedback.fail() end) dataL;
@@ -1111,8 +1197,12 @@ let
         ((rhs o concl) thm1)
    val varL = (fst o strip_forall o rhs o concl) thm1
 
+   val inf_thm = if is_interval then
+                    HOLFOOT_COND_INFERENCE___prog_field_lookup___interval
+                 else
+                    HOLFOOT_COND_INFERENCE___prog_field_lookup___array
    val thm2a = PART_MATCH (snd o dest_imp o snd o dest_imp o snd o dest_imp)
-      (ISPEC t_data HOLFOOT_COND_INFERENCE___prog_field_lookup___array) body_t
+      (ISPEC t_data inf_thm) body_t
    val thm2b = MP thm2a index_thm
    val thm2c = var_res_precondition_prove thm2b
    val thm2d = CONV_RULE ((RATOR_CONV o RAND_CONV o VAR_RES_COND_HOARE_TRIPLE___PRECOND_CONV o
@@ -1237,19 +1327,19 @@ end;
 end;
 
 
+(*
+   val context = map ASSUME (fst (top_goal ()))
+   val tt = find_term is_VAR_RES_COND_HOARE_TRIPLE (snd (top_goal ()))
+*)
 local
-   fun search_fun_array context ec n ttt =
+   fun search_fun_array_interval context ec n ttt =
        let
-          val (e',n',_) = dest_holfoot_ap_data_array ttt
+          val (is_interval, (e',n',_)) = dest_holfoot_ap_data_array_interval ttt
           val nc' = dest_var_res_exp_const n';
           val ec' = dest_var_res_exp_const e';
-
-          val thm_t = mk_conj (
-                         numSyntax.mk_leq (ec', ec),
-                         numSyntax.mk_less (ec, numSyntax.mk_plus (ec', nc')))
-          val thm = array_bound_DECIDE context thm_t
+          val thm = prove_in_array_interval_bound is_interval context ec (ec',nc')
        in          
-          SOME (n, thm, ttt)
+          SOME (n, thm, ttt, is_interval)
        end handle HOL_ERR _ => NONE;
 in
 
@@ -1261,18 +1351,19 @@ let
    val ec = dest_var_res_exp_const e1;
 
    val (_, _, _, _, sfs) = dest_var_res_prop___propL pre;
-   val found_opt = first_opt (search_fun_array context ec) sfs;
+   val found_opt = first_opt (search_fun_array_interval context ec) sfs;
    val _ = if isSome found_opt then () else raise UNCHANGED;
-   val (n, index_thm, sf) = valOf found_opt;
+   val (n, index_thm, sf, is_interval) = valOf found_opt;
 
    (*resort data_entry*)
-   val (_,_,data) = dest_holfoot_ap_data_array sf;
+   val (_, (_,_,data)) = dest_holfoot_ap_data_array_interval sf;
    val (dataL, data_ty) = listSyntax.dest_list data 
    val (dataL2_h, dataL2) = trypluck (fn dt => let val (tag, dl) = pairSyntax.dest_pair dt in
                    if (aconv tag tag_t) then dt else Feedback.fail() end) dataL;
    val data' = listSyntax.mk_list (dataL2_h::dataL2, data_ty)
    val data_perm_thm = EQT_ELIM (permLib.PERM_NORMALISE_CONV (list_mk_icomb (permLib.PERM_tm, [data, data'])))
-   val sf_thm = MATCH_MP (PART_MATCH (lhs o snd o dest_imp) holfoot_ap_data_array___DATA_PERM sf) data_perm_thm
+   val perm_thm = if is_interval then holfoot_ap_data_interval___DATA_PERM else holfoot_ap_data_array___DATA_PERM;
+   val sf_thm = MATCH_MP (PART_MATCH (lhs o snd o dest_imp) perm_thm sf) data_perm_thm
 
    (*resort and apply data_entry_thm*)
    val thm0a = VAR_RES_COND_HOARE_TRIPLE___RESORT_PRECOND_CONV [n] tt;
@@ -1280,8 +1371,11 @@ let
                 (RAND_CONV o RATOR_CONV o RAND_CONV) (K sf_thm)))) thm0a
 
    (*instantiate main theorem*)
-   val thm1a = PART_MATCH (snd o dest_imp o snd o dest_imp)
-      HOLFOOT_COND_INFERENCE___prog_field_assign___array (rhs (concl thm0))
+   val inf_thm = if is_interval then
+        HOLFOOT_COND_INFERENCE___prog_field_assign___interval 
+     else 
+        HOLFOOT_COND_INFERENCE___prog_field_assign___array
+   val thm1a = PART_MATCH (snd o dest_imp o snd o dest_imp) inf_thm (rhs (concl thm0))
    val thm1b = MP thm1a index_thm
    val thm1 = CONV_RULE (RAND_CONV (K (GSYM thm0))) thm1b
 in
@@ -1971,21 +2065,22 @@ end;
 
 
 (* ---------------------------------------- *)
-(* array - same start and length            *)
+(* array / interval - same start and length *)
 (* ---------------------------------------- *)
 
 (*
+   val context = []
    val tt = find_term is_VAR_RES_FRAME_SPLIT (snd (top_goal ()))
 *)
 local 
    fun search_fun sfs n ttt =
        let
-          val (e, ne, _) = dest_holfoot_ap_data_array ttt;
+          val (af, (e, ne, _)) = dest_holfoot_ap_data_array_interval ttt;
           fun search_fun2 m tttt =
           let
-             val (e', ne', _) = dest_holfoot_ap_data_array tttt
+             val (af', (e', ne', _)) = dest_holfoot_ap_data_array_interval tttt
           in
-             if (aconv e e') andalso (aconv ne ne') then
+             if (af' = af) andalso (aconv e e') andalso (aconv ne ne') then
                 SOME (m, tttt)
              else NONE
           end;
@@ -1995,7 +2090,7 @@ local
           let
              val (m, tttt) = valOf found_opt;
           in
-             SOME (n, ttt, m, tttt)
+             SOME (n, ttt, m, tttt, not af)
           end           
        end
 
@@ -2011,7 +2106,7 @@ let
    (*search lists*)
    val found_opt = first_opt (search_fun imp_sfs) split_sfs;
    val _ = if isSome found_opt then () else raise UNCHANGED;
-   val (n, sf1, m, sfb2) = valOf found_opt;
+   val (n, sf1, m, sfb2, af) = valOf found_opt;
 
    (*resort*)
    val thm0 = (VAR_RES_FRAME_SPLIT___split_CONV (BAG_RESORT_CONV [n]) THENC
@@ -2019,9 +2114,11 @@ let
 
 
    (*apply inference*)
-   val thm1 = PART_MATCH (lhs o snd o dest_imp)
-      VAR_RES_FRAME_SPLIT___data_array___data_array___SAME_EXP_LENGTH
-      (rhs (concl thm0))
+   val inf_thm = if af then 
+                    VAR_RES_FRAME_SPLIT___data_array___data_array___SAME_EXP_LENGTH
+                 else 
+                    VAR_RES_FRAME_SPLIT___data_interval___data_interval___SAME_EXP_LENGTH		
+   val thm1 = PART_MATCH (lhs o snd o dest_imp) inf_thm (rhs (concl thm0))
    val thm2 = var_res_precondition_prove thm1
 
    (*undo resorting*)
@@ -2035,45 +2132,62 @@ end;
 
 
 (* ---------------------------------------- *)
-(* array - split if necessary               *)
+(* array / interval - split if necessary    *)
 (* ---------------------------------------- *)
 
 (*
+   val context = map ASSUME (fst (top_goal()))
    val tt = find_term is_VAR_RES_FRAME_SPLIT (snd (top_goal ()))
 *)
 local 
-   val SUB_ADD_SYM = ONCE_REWRITE_RULE [arithmeticTheory.ADD_SYM] 
-        (GSYM arithmeticTheory.SUB_ADD)
+   val array_compset = computeLib.bool_compset ()
+   val _ = computeLib.add_thms [pairTheory.SND, pairTheory.FST, MAP] array_compset
+
+   fun try_split context i1 i2 ec nc1 (nc2,data2) =
+   let
+       val inf_thm = if i1 then 
+          (if i2 then holfoot_ap_data_array_interval___same_start___SPLIT___ii else
+                      holfoot_ap_data_array_interval___same_start___SPLIT___ai) else
+          (if i2 then holfoot_ap_data_array_interval___same_start___SPLIT___ia else
+                      holfoot_ap_data_array_interval___same_start___SPLIT___aa)
+       val xthm0 = ISPECL [ec, nc2, nc1] inf_thm
+       val pre = (fst o dest_imp o snd o strip_forall) (concl xthm0);
+       val pre_thm = array_bound_DECIDE context pre
+
+       val xthm1 = MATCH_MP xthm0 pre_thm;
+       val xthm2 = CONV_RULE ((STRIP_QUANT_CONV o RATOR_CONV o RAND_CONV)
+             (holfoot_arith_simp_CONV context)) xthm1
+       val xthm3 = CONV_RULE (REPEATC Unwind.UNWIND_FORALL_CONV) xthm2
+       val xthm4 = SPEC data2 xthm3
+       val xthm5 = CONV_RULE (RHS_CONV (computeLib.CBV_CONV array_compset)) xthm4
+   in
+      xthm5
+   end;
 
    fun search_fun___same_start context sfs n ttt =
        let
-          val (e, ne, _) = dest_holfoot_ap_data_array ttt;          
+          val (i1, (e, ne, data1)) = dest_holfoot_ap_data_array_interval ttt;          
           val nc1 = dest_var_res_exp_const ne
+          val ec = dest_var_res_exp_const e
           fun search_fun2 m tttt =
           let
-             val (e', ne', _) = dest_holfoot_ap_data_array tttt
+             val (i2, (e', ne', data2)) = dest_holfoot_ap_data_array_interval tttt
+             val _ = if (aconv e e') then () else Feedback.fail ();
+             val nc2 = dest_var_res_exp_const ne'
+             val (in_split, split_thm) = 
+                 (false, try_split context i1 i2 ec nc1 (nc2, data2)) handle HOL_ERR _ =>
+                 (true,  try_split context i2 i1 ec nc2 (nc1, data1))
           in
-             if (aconv e e') andalso (is_var_res_exp_const ne') andalso
-                (not (aconv ne ne')) then
-                (let
-                   val nc2 = dest_var_res_exp_const ne'
-                   val c_t1 = numSyntax.mk_leq (nc1, nc2)
-                   val c_t2 = numSyntax.mk_leq (nc2, nc1)
-                   val (in_split, leq_thm) = (false, array_bound_DECIDE context c_t1) handle HOL_ERR _ =>
-                                             (true,  array_bound_DECIDE context c_t2)
-                in
-                   SOME (m, tttt, in_split, leq_thm)
-                end handle HOL_ERR _ => NONE)
-             else NONE
+             SOME (m, tttt, in_split, split_thm)
           end
           val found_opt = if (is_var_res_exp_const ne) then 
               first_opt search_fun2 sfs else NONE
        in
           if not (isSome found_opt) then NONE else
           let
-             val (m, tttt, in_split, leq_thm) = valOf found_opt;
+             val (m, tttt, in_split, split_thm) = valOf found_opt;
           in
-             SOME (n, m, ttt, tttt, in_split, leq_thm)
+             SOME (n, m, ttt, tttt, in_split, split_thm)
           end           
        end handle HOL_ERR _ => NONE;
 
@@ -2089,28 +2203,12 @@ let
    (*search lists*)
    val found_opt = first_opt (search_fun___same_start context imp_sfs) split_sfs;
    val _ = if isSome found_opt then () else raise UNCHANGED;
-   val (n, m, sf1, sf2, in_split, leq_thm) = valOf found_opt;
-
-   val add_thm0 = MATCH_MP SUB_ADD_SYM leq_thm
-   val arith_simp_CONV = SIMP_CONV arith_ss []
-   val add_thm = CONV_RULE (RHS_CONV (RAND_CONV arith_simp_CONV)) add_thm0
-
-
-   val array_split_thm = let
-      val t0 = if in_split then sf1 else sf2;
-      val xthm0 = RATOR_CONV (RAND_CONV (RAND_CONV (K add_thm))) t0
-      val xthm1 = PART_MATCH (lhs o snd o dest_imp) holfoot_ap_data_array___SPLIT
-         (rhs (concl xthm0));
-      val xthm2 = var_res_precondition_prove xthm1;
-      val xthm3 = TRANS xthm0 xthm2
-
-      val xthm4 = CONV_RULE (RHS_CONV (SIMP_CONV list_ss [])) xthm3
-   in xthm4 end
+   val (n, m, sf1, sf2, in_split, split_thm) = valOf found_opt;
 
 
    (*resort and apply*)
    val array_split_conv = (if in_split then VAR_RES_FRAME_SPLIT___split_CONV else
-                          VAR_RES_FRAME_SPLIT___imp_CONV) (RATOR_CONV (RAND_CONV (K array_split_thm)))
+                          VAR_RES_FRAME_SPLIT___imp_CONV) (RATOR_CONV (RAND_CONV (K split_thm)))
 
    val thm0 = (VAR_RES_FRAME_SPLIT___split_CONV (BAG_RESORT_CONV [n]) THENC
                VAR_RES_FRAME_SPLIT___imp_CONV (BAG_RESORT_CONV [m]) THENC
@@ -2122,36 +2220,29 @@ end;
 end;
 
 
-
+(*
+   val context = map ASSUME (fst (top_goal()))
+   val tt = find_term is_VAR_RES_FRAME_SPLIT (snd (top_goal ()))
+*)
 
 local 
    fun search_fun___not_same_start context sfs n ttt =
        let
-          val (e, ne, _) = dest_holfoot_ap_data_array ttt;          
+          val (is_interval, (e, ne, _)) = dest_holfoot_ap_data_array_interval ttt;          
           val nc1 = dest_var_res_exp_const ne
           val ec1 = dest_var_res_exp_const e
           fun search_fun2 m tttt =
           let
-             val (e', ne', _) = dest_holfoot_ap_data_array tttt
+             val (is_interval', (e', ne', _)) = dest_holfoot_ap_data_array_interval tttt
           in
              if not (aconv e e') then
                 (let
                    val nc2 = dest_var_res_exp_const ne'
                    val ec2 = dest_var_res_exp_const e'
-
-                   fun prove_in_range ec (ec', nc') =
-                   let
-                      val t1 = numSyntax.mk_leq (ec', ec)
-                      val t2 = numSyntax.mk_leq (ec, numSyntax.mk_plus (ec', nc'))
-                      val t3 = mk_conj (t1,t2);
-                      val thm = array_bound_DECIDE context t3
-                   in
-                      thm
-                   end
-                   val (in_split, a_thm) = (false, prove_in_range ec1 (ec2, nc2)) handle HOL_ERR _ =>
-                                           (true,  prove_in_range ec2 (ec1, nc1))
+                   val (in_split, a_thm) = (false, prove_in_array_interval_bound is_interval' context ec1 (ec2, nc2)) handle HOL_ERR _ =>
+                                           (true,  prove_in_array_interval_bound is_interval  context ec2 (ec1, nc1))
                 in
-                   SOME (m, tttt, in_split, a_thm)
+                   SOME (m, tttt, in_split, a_thm, is_interval')
                 end handle HOL_ERR _ => NONE)
              else NONE
           end
@@ -2159,15 +2250,11 @@ local
        in
           if not (isSome found_opt) then NONE else
           let
-             val (m, tttt, in_split, a_thm) = valOf found_opt;
+             val (m, tttt, in_split, a_thm, is_interval') = valOf found_opt;
           in
-             SOME (n, m, ttt, tttt, in_split, a_thm)
+             SOME (n, m, ttt, tttt, in_split, a_thm, is_interval')
           end           
        end handle HOL_ERR _ => NONE;
-
-
-   val sub_add_simp = prove (``(((x:num) + (c1:num)) - (x + c2)) = (c1 - c2)``, DECIDE_TAC)
-
 in
 
 fun VAR_RES_FRAME_SPLIT_INFERENCE___data_array___not_same_start___CONV context tt =
@@ -2180,15 +2267,21 @@ let
    (*search lists*)
    val found_opt = first_opt (search_fun___not_same_start context imp_sfs) split_sfs;
    val _ = if isSome found_opt then () else raise UNCHANGED;
-   val (n, m, sf1, sf2, in_split, a_thm) = valOf found_opt;
+   val (n, m, sf1, sf2, in_split, a_thm, is_interval) = valOf found_opt;
 
 
    val array_split_thm = let
       val t0 = if in_split then sf1 else sf2;
-      val xthm0 = MATCH_MP holfoot_ap_data_array___SPLIT___intro_same_start a_thm
-      val xthm1_pre = (lhs o fst o dest_imp o snd o strip_forall o concl) xthm0
-      val xthm1_pre_thm = SIMP_CONV arith_ss [sub_add_simp] xthm1_pre
-      val xthm1 = MATCH_MP xthm0 xthm1_pre_thm
+      val inf_thm = if is_interval then
+              holfoot_ap_data_interval___SPLIT
+            else holfoot_ap_data_array___SPLIT___intro_same_start
+      val xthm0 = MATCH_MP inf_thm a_thm
+      val xthm1 = if is_interval then xthm0 else
+          let
+             val xthm1_pre = (lhs o fst o dest_imp o snd o strip_forall o concl) xthm0
+             val xthm1_pre_thm = holfoot_arith_simp_CONV context xthm1_pre
+             val xthm1 = MATCH_MP xthm0 xthm1_pre_thm
+          in xthm1 end;
       val xthm2 = PART_MATCH lhs xthm1 t0;
       val xthm3 = CONV_RULE (RHS_CONV (SIMP_CONV list_ss [])) xthm2
    in xthm3 end
@@ -2277,11 +2370,7 @@ local
              val (e', ne', _) = dest_holfoot_ap_data_array tttt
              val nc2 = dest_var_res_exp_const ne'
              val ec2 = dest_var_res_exp_const e'
-
-             val t1 = numSyntax.mk_leq (ec2, ec1)
-             val t2 = numSyntax.mk_leq (ec1, numSyntax.mk_plus (ec2, nc2))
-             val t3 = mk_conj (t1,t2);
-             val thm = array_bound_DECIDE context t3
+             val thm = prove_in_array_bound context ec1 (ec2, nc2);
           in
              SOME (m, tttt)
           end handle HOL_ERR _ => NONE)
@@ -2514,6 +2603,14 @@ val HF_ELIM_COMMENTS_TAC = VAR_RES_ELIM_COMMENTS_TAC;
 val HF_PURE_VC_TAC = VAR_RES_PURE_VC_TAC;
 val HF_VC_TAC = VAR_RES_VC_TAC;
 
+fun xHF_SIMPLIFY_TAC optL = xHF_STEP_TAC_n optL 3 (SOME 0);
+val HF_SIMPLIFY_TAC = xHF_SIMPLIFY_TAC [];
+
+
+fun HF_INIT_TAC (asm, t) = 
+  (if (is_FASL_SPECIFICATION t) then VAR_RES_SPECIFICATION_TAC else
+  VAR_RES_ENTAILMENT_INIT_TAC) (asm, t)
+
 
 fun print s = Portable.output(Portable.std_out, s)
 
@@ -2522,15 +2619,19 @@ fun holfoot_set_goal file =
 
 fun holfoot_set_goal_preprocess file =
    ((proofManagerLib.set_goal([], parse_holfoot_file file));
-    (proofManagerLib.e (HF_SPECIFICATION_TAC));
+    (proofManagerLib.e (HF_INIT_TAC));
     (proofManagerLib.forget_history());
     (proofManagerLib.status()));
 
 fun holfoot_set_goal_procedures file fL =
    ((proofManagerLib.set_goal ([], parse_holfoot_file_restrict fL file));
-   (proofManagerLib.e (HF_SPECIFICATION_TAC THEN REPEAT CONJ_TAC));
+   (proofManagerLib.e (HF_INIT_TAC THEN REPEAT CONJ_TAC));
    (proofManagerLib.forget_history());
    (proofManagerLib.status ()));
+
+val holfoot_set_goal_specs = holfoot_set_goal_procedures;
+
+
 
 fun print_space n = if n > 0 then (print " ";print_space (n-1)) else ()
 
@@ -2603,18 +2704,32 @@ fun holfoot_verify_spec_internal verbose print_remaining (file, defaultConseqCon
                          ("\nparsing ... "))
 
      val t = parse_holfoot_file file;    
+     val is_spec = is_FASL_SPECIFICATION t
 
      val _ = if verbose then (print_timer true (true,false); print "\n\n"; print_backend_term t; print "\n\n")
                         else (print "\n");
 
      val procedure_names =
+     if (is_spec) then
      let
         val tL = (fst o listSyntax.dest_list o rand) t;
         val ntL = map (el 2 o pairSyntax.strip_pair) tL;
         val nL = map stringLib.fromHOLstring ntL
      in
         nL
-     end;
+     end else 
+     let
+        val tL = strip_conj t
+        val e = el 1 tL
+        fun get_comment e =
+           let
+              val (_, rfc, _, _, _, _, _, _) = dest_VAR_RES_FRAME_SPLIT e;
+              val s = (fst o dest_var o rand o rator o rand o rand) rfc
+           in s end;
+        val nL = map get_comment tL
+     in
+        nL
+     end
 
      val max_width = foldl (fn (a,b:int) => if a > b then a else b) 23 (map (fn s => size s + 5) procedure_names)
      fun print_dots false s = ()
@@ -2622,14 +2737,14 @@ fun holfoot_verify_spec_internal verbose print_remaining (file, defaultConseqCon
 
      val _ = start_timer ();
      val _ = print_dots verbose "preprocessing";   
-     val thm_spec = HF_SPECIFICATION_CONSEQ_CONV t;
+     val thm_spec = if is_spec then HF_SPECIFICATION_CONSEQ_CONV t else
+                    VAR_RES_ENTAILMENT_INIT___CONSEQ_CONV t;
      val _ = print_timer verbose (true, false)
 
-     val _ = if (verbose) then (print_dots true "verifying specification";print "\n") else ();
-     val procedure_conds = (strip_conj o fst o dest_imp o concl) thm_spec
-     val pc = hd procedure_conds
-     fun verify_proc pc = let
-        val p_name = (fst o dest_var o rand o rator o rand o rator) (find_term is_fasl_comment_location pc)
+     val _ = if (verbose) then (print_dots true (if is_spec then "verifying specification" else "verifying entailments");print "\n") else ();
+     val procedure_conds = zip procedure_names
+            ((strip_conj o fst o dest_imp o concl) thm_spec)
+     fun verify_proc (p_name, pc) = let
         val my_TAC_opt = SOME (Lib.assoc p_name tacL) handle HOL_ERR _ => NONE
         val _ = print_dots verbose ("   * "^p_name);
         val _ = start_timer();
