examples/separationLogic/src/separationLogicSyntax.sml
@@ -152,6 +152,7 @@ fun mk_FASL_PROGRAM_IS_ABSTRACTION (xenv,penv,x,y) =
 
 val FASL_SPECIFICATION_term = asl_mk_const "FASL_SPECIFICATION"
 val dest_FASL_SPECIFICATION = strip_comb_3 FASL_SPECIFICATION_term;
+val is_FASL_SPECIFICATION = can dest_FASL_SPECIFICATION;
 
 
 val COND_PROP___IMP_term = asl_mk_const "COND_PROP___IMP";
@@ -220,6 +221,15 @@ val is_asl_trivial_cond = (can dest_asl_trival_cond);
 
 val dest_asl_star = strip_comb_3 asl_star_term;
 val is_asl_star = (can dest_asl_star);
+fun strip_asl_star t =
+let
+   val (_, p1, p2) = dest_asl_star t;
+   val p1L = strip_asl_star p1;
+   val p2L = strip_asl_star p2;
+in
+   (p1L @ p2L)
+end handle HOL_ERR _ => [t];
+
 
 fun dest_asl_exists tt =
   let
